src/tools/lifter/bir_lifter_general_auxScript.sml
@@ -1,4 +1,7 @@
 open HolKernel Parse boolLib bossLib;
+open sortingTheory listTheory
+open bir_programTheory
+open HolBACoreSimps
 
 (* This theory contains auxiliary definitions
    and lemmata used by the lifter which don't
@@ -72,6 +75,91 @@ val COMBINE_TWO_STEP_THMS_SIMPLE = store_thm ("COMBINE_TWO_STEP_THMS_SIMPLE",
 
 REPEAT STRIP_TAC >>
 Cases_on `cond2` >> FULL_SIMP_TAC std_ss [PROTECTED_COND_def]);
+
+
+
+(***************************************)
+(* Show that set of labels is distinct *)
+(***************************************)
+
+(* If we show naively that the set of labels of a program is distinct,
+   we need quadratic time in the length of the program. It is very slow.
+   We need something more fancy. The lifter produces labels in an ordered
+   form. We can just translate address labels to ints and check that these are
+   sorted. This is much faster. For string labels, we can't do much, though. *)
+
+val bir_labels_of_program_EVAL = store_thm ("bir_labels_of_program_EVAL",
+ ``(bir_labels_of_program (BirProgram []) = []) /\
+   (bir_labels_of_program (BirProgram (bl::bls)) =
+    bl.bb_label :: (bir_labels_of_program (BirProgram bls)))``,
+SIMP_TAC list_ss [bir_programTheory.bir_labels_of_program_def])
+
+
+val ALL_DISTINCT_lifter_labels_list_PART_def = Define `
+(ALL_DISTINCT_lifter_labels_list_PART nl sl [] = (nl, sl)) /\
+(ALL_DISTINCT_lifter_labels_list_PART nl sl ((BL_Address i)::ls) <=> (
+   ALL_DISTINCT_lifter_labels_list_PART ((b2n i)::nl) sl ls)) /\
+(ALL_DISTINCT_lifter_labels_list_PART nl sl ((BL_Label s)::ls) <=> (
+   ALL_DISTINCT_lifter_labels_list_PART nl (s::sl) ls))`;
+
+
+val PERM_PARTITION = store_thm ("PERM_PARTITION",
+``!P l. PERM (FILTER P l ++ FILTER (\x. ~(P x)) l) l``,
+
+GEN_TAC >>
+Induct >- (
+  SIMP_TAC list_ss [PERM_REFL]
+) >>
+GEN_TAC >>
+rename1 `x::xs` >>
+Cases_on `P x` >- (
+  ASM_SIMP_TAC list_ss [PERM_CONS_IFF]
+) >- (
+  ASM_SIMP_TAC list_ss [PERM_FUN_APPEND_CONS, PERM_CONS_IFF]
+));
+
+val ALL_DISTINCT_lifter_labels_list_PART_ALT_DEF = store_thm ("ALL_DISTINCT_lifter_labels_list_PART_ALT_DEF",
+``!ll nl sl.
+  ALL_DISTINCT_lifter_labels_list_PART nl sl ll =
+  ((REVERSE (MAP (\ll. case ll of BL_Address a => b2n a) (FILTER IS_BL_Address ll))) ++ nl,
+   (REVERSE (MAP (\ll. case ll of BL_Label s => s) (FILTER (\l. ~(IS_BL_Address l)) ll))) ++ sl)``,
+
+Induct >- (
+  SIMP_TAC list_ss [ALL_DISTINCT_lifter_labels_list_PART_def]
+) >>
+Cases >> (
+  ASM_SIMP_TAC (list_ss++bir_TYPES_ss) [ALL_DISTINCT_lifter_labels_list_PART_def,
+    IS_BL_Label_def, IS_BL_Address_def] >>
+  SIMP_TAC std_ss [GSYM APPEND_ASSOC, APPEND]
+));
+
+
+val ALL_DISTINCT_lifter_label_list_PARTS_THM = store_thm ("ALL_DISTINCT_lifter_label_list_PARTS_THM",
+``!ll nl sl.
+  (ALL_DISTINCT_lifter_labels_list_PART [] [] ll = (nl, sl)) ==>
+  (ALL_DISTINCT sl /\  SORTED ($>) nl) ==>
+  ALL_DISTINCT ll``,
+
+REPEAT STRIP_TAC >>
+FULL_SIMP_TAC list_ss [ALL_DISTINCT_lifter_labels_list_PART_ALT_DEF] >>
+Q.SUBGOAL_THEN `ALL_DISTINCT ll =
+  ALL_DISTINCT ((FILTER IS_BL_Address ll) ++ (FILTER (\x. ~(IS_BL_Address x)) ll))` SUBST1_TAC >- (
+
+  MATCH_MP_TAC ALL_DISTINCT_PERM >>
+  ONCE_REWRITE_TAC [PERM_SYM] >>
+  METIS_TAC[PERM_PARTITION]
+) >>
+
+`ALL_DISTINCT nl` by (
+  IRULE_TAC SORTED_ALL_DISTINCT >>
+  Q.EXISTS_TAC `$>` >>
+  ASM_SIMP_TAC arith_ss [relationTheory.irreflexive_def,
+    relationTheory.transitive_def]
+) >>
+REPEAT (BasicProvers.VAR_EQ_TAC) >>
+FULL_SIMP_TAC list_ss [ALL_DISTINCT_REVERSE, ALL_DISTINCT_APPEND,
+  MEM_FILTER] >>
+METIS_TAC[ALL_DISTINCT_MAP])
 
 
 val _ = export_theory();
